<head>
    <script src="https://cdn.mathjax.org/mathjax/latest/MathJax.js?config=TeX-AMS-MML_HTMLorMML" type="text/javascript"></script>
    <script type="text/x-mathjax-config">
        MathJax.Hub.Config({
            tex2jax: {
            skipTags: ['script', 'noscript', 'style', 'textarea', 'pre'],
            inlineMath: [['$','$']]
            }
        });
    </script>
</head>

## Differential Equations

![](img_1.png)

In Newton's second law
- t is independent variable
- x is dependent variable

Difference between ODE and PDE:
- ODE's unknown function depends on only one independent varibale while the one of PDE depends on more than one independent varibale

#### Example of PDE and partial derivatives
- unknown function $f(x,y)$ has two independent variable $x$ and $y$
- partial derivative
	- first order - $\frac{\partial f}{\partial x}$ and $\frac{\partial f}{\partial y}$
	- second order - $\frac{\partial^2 f}{\partial x^2}$, $\frac{\partial^2 f}{\partial y^2}$ and $\frac{\partial^2 f}{\partial x\partial y}$ 

## Linear DEs

![](img_2.png)

## Solutions of DEs and Initial Value Problems

![](img_3.png)

**General Solution** has to include all solution of given DE

**Initial condition** and **boundary condition** are called **side conditions** 

**Rule of Thumb**:
- the order of a DE $=$ of side conditions of DE

#### Examples of IVP and BVP

- IVP - given value at same $t$ where $t = 0$

$$\begin{cases}
2x^{''} = x(t) \\
x(0) = 1 \\
x^{'}(0) = 2
\end{cases}$$

-BVP - given value at different $t$

$$\begin{cases}
2x^{''} = x(t) \\
x(0) = 1 \\
x(1) = 2
\end{cases}$$

## The Simplest DEs: Antiderivatives

![](img_4.png)

Another way to write the general solution using a definite integral, where $y(t_0)$ is same as $C$

$$y(t) - y(t_0) = \int_{t_0}^{t} g(s)ds$$

And $y(t_0) = y_0$ is a given inital condition

### Example

![](img_5.png)

## First-order linear ODEs

![](img_6.png)

### The integrating factor method

![](img_7.png)

**Side Note**:

$$ \mu = e^{\int p(t)dt}$$
$$ \mu (y^{'}(t) + p(t)y(t) = \mu g(t) $$
$$ \mu y^{'}(t) + \mu p(t)y(t) = \mu g(t)$$

Taking derivate of integral of a function equals to the function itself

$$ \because \mu^{'} = \frac{d}{dt} e^{\int p(t)dt} = p(t) e^{\int p(t)dt}$$
$$ \therefore \mu y^{'}(t) + \mu^{'}y(t) = \mu g(t) $$

by mupltiplication

$$ \frac{d}{dt}(\mu (t) y(t)) = \mu g(t)$$
